\input{header.tex}
\setcounter{theorem}{4}
\begin{exercise} BH.8.5
\begin{solution}
Use the mnemonic of exercise BH.8.1 to get the order of $\d y/\d x$ right.

Now note that $|Z|=z \implies X = z$ or $X=-z$ for $z>0$.  Also, $|\d z/\d x| = 1$  for $z>0$. Therefore,
\begin{align*}
  f_{Z}(z) = f_{X}(-z)  + f_X(z) \stackrel1 = 2f_X(z) = 2\phi(z),
\end{align*}
where step 1 follows from the symmetry of $\Norm{0, \sigma}$ under reflection in the $y$-axis. Since $\int_0^0 f_X(x) \d x = 0$, we can take any value we like for $f_{Z}(z)$ for $z=0$, so why not $2 \phi(0)$ too? And thus,
\begin{align*}
  f_{Z}(z) = f_{X}(-z)  + f_X(z) \stackrel1 = 2f_X(z) = 2\phi(z), \quad z \geq 0.
\end{align*}
Of course $\phi$ is the density of the standard normal distribution.
\end{solution}
\end{exercise}
\input{trailer.tex}
