\input{header.tex}
\setcounter{theorem}{12}
\begin{exercise}BH.8.13
\begin{hint}
Note that the following implications hold:
\begin{align*}
\{T\leq t\} = \{X/Y \leq e^{t}\} = \{X \leq e^t Y\}
\end{align*}
\end{hint}
\begin{solution}
With the hint:
\begin{align*}
\P{T\leq t}
  &= \P{X \leq e^t Y} = \lambda \int_0^{\infty} \P{X\leq e^{t}y} e^{-\lambda y} \d y
  = \lambda \int_0^{\infty} (1- \exp{(-\lambda e^{t} y)}) e^{-\lambda y}\d y \\
&= 1 - \lambda \int_0^{\infty} \exp{(-\lambda (e^{t}+1) y)} \d y = 1-\frac{\lambda}{\lambda(e^{t}+1)}.
\end{align*}
Clearly, we can cancel the $\lambda$. For the PDF, just take the derivative with respect to $t$.
\end{solution}
\end{exercise}
\input{trailer.tex}
